high2/Zeta.High.Interleave.fsti
@@ -13,6 +13,7 @@ module V = Zeta.GenericVerifier
 module T = Zeta.Generic.Thread
 module G = Zeta.Generic.Global
 module GI = Zeta.Generic.Interleave
+module HV = Zeta.High.Verifier
 module I = Zeta.Interleave
 module S = FStar.Seq
 module SA = Zeta.SeqAux
@@ -31,6 +32,12 @@ let verifiable_log (app:_) (n:nat)
 let thread_store (#app #n:_) (tid: nat{tid < n}) (il: verifiable_log app n)
   = let vs = thread_state tid il in
     vs.st
+
+let has_some_add_of_key (#app #n:_) (bk: base_key) (il: verifiable_log app n)
+  = exists i. HV.is_add_of_key bk (I.index il i)
+
+let exists_in_some_store (#app #n:_) (bk: base_key)  (il: verifiable_log app n)
+  = exists tid. store_contains (thread_store tid il) bk
 
 val mk_vlog_entry_ext (#app: app_params) (#n:nat)
   : IF.idxfn_t (gen_seq app n) (vlog_entry_ext app)
@@ -53,13 +60,23 @@ val is_eac (#app #n:_) (il: verifiable_log app n)
 val eac_state_of_key (#app #n:_) (k: base_key)
   : IF.seqfn_t (gen_seq app n) (eac_state app k)
 
+let eac_state_of_gkey (#app #n:_) (gk: key app) (il: verifiable_log app n)
+  : (eac_state app (to_base_key gk))
+  = let bk = to_base_key gk in
+    eac_state_of_key bk il
+
 (* is the key k in evicted state in *)
 let is_eac_state_evicted (#app #n:_) (k: base_key) (il: verifiable_log app n): bool
   = EACEvictedMerkle? (eac_state_of_key k il) ||
     EACEvictedBlum? (eac_state_of_key k il)
 
-val eac_value (#app #n:_) (gk: key app)
-  : IF.seqfn_t (gen_seq app n) (value_t gk)
+let is_eac_state_active (#app #n:_) (k: base_key) (il: verifiable_log app n)
+  = let es = eac_state_of_key k il in
+    es <> EACInit && es <> EACFail
+
+let is_eac_state_active_gk (#app #n:_) (gk: key app) (il: verifiable_log app n)
+  = let es = eac_state_of_gkey gk il in
+    es <> EACInit && es <> EACFail
 
 val empty_implies_eac (#app #n:_) (il: verifiable_log app n)
   : Lemma (ensures (length il = 0 ==> is_eac il))
@@ -71,13 +88,6 @@ val eac_state_transition (#app #n:_) (k: base_key)
                     let smk = eac_smk app k in
                     let ee = mk_vlog_entry_ext il i in
                     es_post = eac_add ee es_pre))
-
-val eac_implies_eac_state_valid (#app #n:_) (k: base_key)
-  (il: verifiable_log app n)
-  : Lemma (ensures (is_eac il ==> eac_state_of_key k il <> EACFail))
-
-val eac_state_of_root_init (#app #n:_) (il: verifiable_log app n)
-  : Lemma (ensures (eac_state_of_key Zeta.BinTree.Root il = EACInit))
 
 let eac_log (app: app_params) (n:nat) = il: verifiable_log app n {is_eac il}
 
@@ -91,6 +101,60 @@ val lemma_eac_implies_appfn_calls_seq_consistent (#app #n:_) (il: eac_log app n)
   : Lemma (ensures (let gl = to_glog il in
                     Zeta.AppSimulate.seq_consistent (G.appfn_calls gl)))
 
+val eac_implies_eac_state_valid (#app #n:_) (k: base_key)
+  (il: verifiable_log app n)
+  : Lemma (ensures (is_eac il ==> eac_state_of_key k il <> EACFail))
+
+val eac_state_of_root_init (#app #n:_) (il: eac_log app n)
+  : Lemma (ensures (eac_state_of_key Zeta.BinTree.Root il = EACInit))
+
+val eac_state_active_implies_prev_add (#app #n:_) (k: base_key) (il: eac_log app n)
+  : Lemma (ensures (is_eac_state_active k il <==> has_some_add_of_key k il))
+
+(* when the eac_state of k is instore, then k is in the store of a unique verifier thread *)
+val stored_tid (#app:_) (#n:nat) (k: base_key) (il: eac_log app n {EACInStore? (eac_state_of_key k il)})
+  : tid:nat{tid < n /\ store_contains (thread_store tid il) k}
+
+val lemma_instore (#app #n:_) (bk: base_key) (il: eac_log app n)
+  : Lemma (ensures (exists_in_some_store bk il <==> EACInStore? (eac_state_of_key bk il)))
+
+(* uniqueness: k is never in two stores *)
+val key_in_unique_store (#app #n:_) (k:base_key) (il: eac_log app n) (tid1 tid2: thread_id il)
+  : Lemma (ensures (tid1 <> tid2 ==>
+                    ~ (store_contains (thread_store tid1 il) k /\ store_contains (thread_store tid2 il) k)))
+
+val to_gen_key (#app #n:_) (bk: base_key) (il: eac_log app n {is_eac_state_active bk il})
+  : gk:key app {to_base_key gk = bk}
+
+val stored_key_is_correct (#app #n:_) (bk: base_key) (il: eac_log app n{EACInStore? (eac_state_of_key bk il)})
+  : Lemma (ensures (let tid = stored_tid bk il in
+                    let st = thread_store tid il in
+                    stored_key st bk = to_gen_key bk il))
+
+let stored_value (#app #n:_) (gk: key app) (il: eac_log app n{EACInStore? (eac_state_of_gkey gk il)})
+  : value_t gk
+  = let bk = to_base_key gk in
+    let tid = stored_tid bk il in
+    let st = thread_store tid il in
+    stored_value st bk
+
+let stored_add_method (#app #n:_) (gk: key app) (il: eac_log app n{EACInStore? (eac_state_of_gkey gk il)})
+  : add_method
+  = let bk = to_base_key gk in
+    let tid = stored_tid bk il in
+    let st = thread_store tid il in
+    add_method_of st bk
+
+(* the root is always in thread 0 *)
+val lemma_root_in_store0 (#app #n:_) (il: verifiable_log app n)
+  : Lemma (requires (n > 0))
+          (ensures (store_contains (thread_store 0 il) Zeta.BinTree.Root))
+
+val lemma_root_not_in_store (#app #n:_) (tid: nat{tid < n /\ tid > 0}) (il: verifiable_log app n)
+  : Lemma (not (store_contains (thread_store tid il) Zeta.BinTree.Root))
+
+val eac_value (#app #n:_) (k: key app) (il: eac_log app n)
+  : value_t k
 
 val eac_boundary (#app #n:_) (il: neac_log app n)
   : (i: seq_index il{is_eac (prefix il i) /\
